---
author: Math 51 Fall 2021
title: |
  Worksheet for week 10 - some solutions
date: 2022-04-01
bibliography: 
 - /home/george/Prof-Math/assets/math-bibliography.bib
 - /home/george/Prof-Math/assets/teaching.bib 
csl: assets/chicago-author-date.csl
header-includes: |
  \usepackage[top=25mm,bottom=25mm,left=25mm,right=25mm]{geometry}
---

Concerning problem 6.

Write $A = \begin{bmatrix} 1 & 1 & 0 & 0 \\ -1 & 1 & 1 & 0 \\ 0 & 0 &
1 & -1 \\ 0 & 0 & 1 & 1 \end{bmatrix} =\begin{bmatrix} B & C \\ 0 &
B^t \end{bmatrix}$ where $$B = \begin{bmatrix} 1 & 1 \\ -1 & 1
\end{bmatrix}, \quad C = \begin{bmatrix} 0 & 0 \\ 1 & 0
\end{bmatrix}$$ and $B^t$ is the *transpose* of $B$.

Since $A$ is *block upper triangular*, the char. poly of $A$ is given
by $$\det(A - \lambda I) = \det \begin{bmatrix} B-\lambda I & C \\ 0 &
B^t - \lambda I \end{bmatrix} = \det (B - \lambda I) \det (B^t -
\lambda I) = \det(B - \lambda I)^2.$$

(This last equality holds because $\det M = \det M^t$ for any square matrix $M$
and because $(M-\lambda I)^t = M^t - \lambda I$).

Now, $\det (B - \lambda I)= \det \begin{bmatrix} 1-\lambda & 1 \\ -1 & 1-\lambda
\end{bmatrix} = (1-\lambda)^2 + 1 = \lambda^2 - 2\lambda + 2.$

Thus the characteristic polynomial of $A$ is $(\lambda^2 - 2\lambda +
2)^2$. In particular, using the quadratic formula we see that $A$ has
eigenvalues $1 + i$ (with multiplicity 2) and $1-i$ (with multiplicity
2).

If we now try to find eigenvectors, we will find that there is only
one linearly independent $1+i$ eigenvector, and only 1 linearly
independent $1-i$ eigenvector. So to find the general solution $Dx =
Ax$ we find generalized eigenvectors.

Thus we need to find solutions to $(A-(1+i))^2x = 0$. We start by computing
$(A-(1+i))^2$ and putting the result in echelon form using row operations:

\begin{align*}
(A-(1+i))^2 &= \begin{bmatrix}
-i & 1 & 0 & 0 \\
-1 & -i & 1 & 0 \\ 
0 & 0 & -i & -1 \\
0 & 0 & 1 & -i
\end{bmatrix} \cdot 
\begin{bmatrix}
-i & 1 & 0 & 0 \\
-1 & -i & 1 & 0 \\ 
0 & 0 & -i & -1 \\
0 & 0 & 1 & -i
\end{bmatrix}
=
\begin{bmatrix}
-2 & -2i & 1 & 0 \\
2i & -2 & -2i & -1 \\
0 & 0 & -2 & 2i \\
0 & 0 & -2i & -2
\end{bmatrix} \\
&\sim 
\begin{bmatrix}
2 & 2i & -1 & 0 \\
2 & 2i & -2 & i \\
0 & 0 & 2 & -2i \\
0 & 0 & 2 & -2i
\end{bmatrix}
\sim 
\begin{bmatrix}
2 & 2i & -1 & 0 \\
0 & 0 & -1 & i \\
0 & 0 & 1 & -i \\
0 & 0 & 0 & 0
\end{bmatrix} \\
&\sim 
\begin{bmatrix}
2 & 2i & -1 & 0 \\
0 & 0 & 1 & -i \\
0 & 0 & 0 & 0 \\
0 & 0 & 0 & 0
\end{bmatrix}
\sim 
\begin{bmatrix}
2 & 2i & 0 &-i \\
0 & 0 & 1 & -i \\
0 & 0 & 0 & 0 \\
0 & 0 & 0 & 0
\end{bmatrix}
\end{align*}

We find now that solutions to $(A-(1+i))^2x = 0$ are generated by the
vectors $$\mathbf{v}_1 = \begin{bmatrix} i/2 \\ 0 \\ i \\ 1
\end{bmatrix} \quad \text{and} \quad \mathbf{v}_2 = \begin{bmatrix} -i
\\ 1 \\ 0 \\ 0 \end{bmatrix}$$ -- i.e. $\mathbf{v}_1$ and
$\mathbf{v}_2$ generate the generalized eigenvectors for $\lambda =
1+i$.

Let's compute
$$(A-(1+i))\mathbf{v}_1 = \begin{bmatrix}
-i & 1 & 0 & 0 \\
-1 & -i & 1 & 0 \\ 
0 & 0 & -i & -1 \\
0 & 0 & 1 & -i
\end{bmatrix} \begin{bmatrix} i/2 \\ 0 \\ i \\ 1
\end{bmatrix}
= \begin{bmatrix} 1/2 \\ i/2 \\ 0 \\ 0
\end{bmatrix}$$

and

$$(A-(1+i))\mathbf{v}_2 = \begin{bmatrix}
-i & 1 & 0 & 0 \\
-1 & -i & 1 & 0 \\ 
0 & 0 & -i & -1 \\
0 & 0 & 1 & -i
\end{bmatrix} \begin{bmatrix} -i \\ 1 \\ 0 \\ 0
\end{bmatrix}
= \begin{bmatrix} 0 \\ 0 \\ 0 \\ 0 
\end{bmatrix}$$
Thus $\mathbf{v}_2$ is an *actual* eigenvector.

We now find complex solutions
$$\mathbf{h}_1(t) = e^{(1+i)t}  \left (
\begin{bmatrix} i/2 \\ 0 \\ i \\ 1
\end{bmatrix}
+t \begin{bmatrix} 1/2 \\ i/2 \\ 0 \\ 0
\end{bmatrix} \right ) \quad
= \dfrac{e^{(1+i)t}}{2} \cdot \begin{bmatrix}
i + t \\ it \\ 2i \\ 2
\end{bmatrix} \quad \text{and} \quad 
\mathbf{h}_2(t) = e^{(1+i)t} 
\begin{bmatrix} -i \\ 1 \\ 0 \\ 0
\end{bmatrix}$$

To find the general solution to $Dx = Ax$, it remains to find the
*real* and *imaginary* parts of $\mathbf{h}_1(t)$ and of
$\mathbf{h}_2(t)$.

We have
\begin{align*}
\mathbf{h}_1(t) &= \dfrac{e^{(1+i)t}}{2} \cdot \begin{bmatrix}
i + t \\ it \\ 2i \\ 2
\end{bmatrix}
= \dfrac{e^t}{2}(\cos(t) + i \sin(t))
 \begin{bmatrix}
i + t \\ it \\ 2i \\ 2
\end{bmatrix}
= \dfrac{e^t}{2}
 \begin{bmatrix}
-\sin(t) + i\cos(t) + t(\cos(t) + i\sin(t)) \\ t(-\sin(t)+i\cos(t)) \\ 2(-\sin(t)+i\cos(t)) \\ 2(\cos(t) + i \sin(t))
\end{bmatrix} \\
&= \dfrac{e^t}{2}\begin{bmatrix}   -\sin(t) +t\cos(t) \\ -t\sin(t) \\-2\sin(t) \\ 2\cos(t) \end{bmatrix}
 + \dfrac{ie^t}{2}\begin{bmatrix} \cos(t) + t\sin(t) \\ t\cos(t) \\ 2\cos(t) \\ 2\sin(t) \end{bmatrix}
\end{align*}

$$\mathbf{h}_2(t) = e^{(1+i)t} 
\begin{bmatrix} -i \\ 1 \\ 0 \\ 0
\end{bmatrix}
= e^t(\cos(t) + i \sin(t))
\begin{bmatrix} -i \\ 1 \\ 0 \\ 0
\end{bmatrix}
= 
e^t\begin{bmatrix} \sin(t) -i \cos(t) \\ 
\cos(t) + i \sin(t) \\ 0 \\ 0
\end{bmatrix}
= 
e^t\begin{bmatrix} \sin(t) \\ \cos(t) \\ 0 \\ 0 
\end{bmatrix}
 + 
i e^t\begin{bmatrix} -\cos(t) \\ \sin(t) \\ 0 \\ 0 
\end{bmatrix} 
$$

Thus the general solution to $Dx = Ax$ is given by
$$c_1 e^t\begin{bmatrix}   -\sin(t)+t\cos(t) \\ -t\sin(t) \\-2\sin(t) \\ 2\cos(t) \end{bmatrix}
+ c_2 e^t\begin{bmatrix} \cos(t)+t\sin(t) \\ t\cos(t) \\ 2\cos(t) \\ 2\sin(t) \end{bmatrix}
+ c_3 e^t\begin{bmatrix} \sin(t) \\ \cos(t) \\ 0 \\ 0 
\end{bmatrix} 
+ c_4 e^t\begin{bmatrix} -\cos(t) \\ \sin(t) \\ 0 \\ 0 
\end{bmatrix}$$
