---
author: George McNinch (Math 51 Spring 2022)
title: Week 12 - The Laplace Transform
date: 2022-04-13
bibliography: 
 - /home/george/Prof-Math/assets/math-bibliography.bib
 - /home/george/Prof-Math/assets/teaching.bib
csl: assets/chicago-author-date.csl
header-includes: |
  \usepackage[top=25mm,bottom=25mm,left=25mm,right=25mm]{geometry}
---

This lecture follows [@gutermanNitecki, sec. 5.2 & 5.3].

# The Laplace Transform

## Definition of the Laplace transform

Consider a function $f(t)$ of the variable $t$. The **Laplace
transform** of $f(t)$ is a *new function* $F(s)$ of a *new variable*
$s$ defined by the formula

$$F(s) = \int_0^\infty e^{-st} f(t) dt.$$

. . .

We write 
$$\mathscr{L}[f(t)] = \mathscr{L}[f(t)](s) = F(s)$$
for this function.

-----

::: incremental 
- we emphasize: 

  - the *input* of $\mathscr{L}$ is a function of $t$, and 
  - the *output* of $\mathscr{L}$ is a function of $s$.
  
- the indefinite integral defining $F(s)$ is taken with respect to $t$
  (i.e. we integrate "$dt$"):

  $$F(s) = \int_0^\infty e^{-st} f(t) dt = \lim_{h \to \infty} \int_0^h e^{-st}f(t)dt.$$

  In this integral, the variable $s$ *can be treated like a scalar*.

- we are going to derive *formulas* for several families of functions
  $f(t)$ which will permit us calculate $\mathscr{L}[f]$.

- then, we are going to use the Laplace transform to solve *initial value
  problems* arising from certain ODEs.


:::


## Basic Laplace transforms

Let's first list some Laplace transforms, and then we'll check a few
of the *derivations*.

::: incremental

- $\mathscr{L}[e^{\lambda t}] = \dfrac{1}{s-\lambda}$ for $s > \lambda$

- $\mathscr{L}[1] = \dfrac{1}{s}$ for  $s > 0$

- $\mathscr{L}[t^n] = \dfrac{n!}{s^{n+1}}$ for $s>0$.

- $\mathscr{L}[\sin(\beta t)] = \dfrac{\beta}{s^2 + \beta^2}$ for $s>0$.

- $\mathscr{L}[\cos(\beta t)] = \dfrac{s}{s^2 + \beta^2}$ for $s>0$.

- **Remark:** Notice that for these functions $f$, the Laplace
transform $\mathscr{L}[f] = F(s)$ is always defined "for all large
enough values of $s$" - i.e. for all $s$ in some interval
$(N,\infty)$.

::: 


## check: $\mathscr{L}[e^{\lambda t}]$

$$\mathscr{L}[e^{\lambda t}](s) = \lim_{h \to \infty} \int_0^h
 e^{-st} e^{\lambda t} dt = \lim_{h \to \infty} \int_0^h e^{-(s - \lambda)t} dt  \quad (\clubsuit)$$

::: incremental


- Now if $\lambda \ne s$, then $$\displaystyle \int_0^h
  e^{-(s-\lambda)t} dt = \dfrac{-1}{s-\lambda} e^{-(s-\lambda )t}
  \bigg \vert^h_0 = \dfrac{-1}{s- \lambda} [e^{-(s-\lambda)h} - 1] =
  \dfrac{1}{s-\lambda} - e^{-(s-\lambda)h} \dfrac{1}{s-\lambda}$$

- If $\lambda < s$ then $\displaystyle \lim_{h \to \infty}
  e^{-(s-\lambda)h} = 0$ and we see that $(\clubsuit) =
  \dfrac{1}{s-\lambda}$.

- This confirms that $\mathscr{L}[e^{\lambda t}](s) =
  \dfrac{1}{s-\lambda}$

- Notice that if $\lambda = 0$ then $e^{\lambda t} = 1$ and we get
  $\mathscr{L}[1] = \dfrac{1}{s}$.

:::

## Check: $\mathscr{L}[t^n]$, $n \ge 1$.

::: incremental

- Integration by parts with $u = t^n$ and $dv = e^{-st}dt$ gives

  $$\int_0^h e^{-st}t^n dt = \dfrac{-h^n e^{-sh}}{s} + \dfrac{n}{s} \int_0^h e^{-st} t^{n-1} dt$$ 
  
- as $h \to \infty$, the *left-hand-side* approaches $\mathscr{L}[t^n](s)$. If $s > 0$, then
  l'HÃ´pital's rule shows that the first term on the right goes to 0, while the second
  term approaches $\dfrac{n}{s}\mathscr{L}[t^{n-1}]$.
  
- conclude that for $s>0$ and $n>0$, we have $(\heartsuit) \quad
  \mathscr{L}[t^n] = \dfrac{n}{s}\mathscr{L}[t^{n-1}]$.

- we know that $\mathscr{L}[t^0] = \mathscr{L}[1] = \dfrac{1}{s}$.

- we get $\mathscr{L}[t] = \dfrac{1}{s}\mathscr{L}[t^0] = \dfrac{1}{s^2}.$


:::

----

::: incremental

- and now we can bootstrap using the previous fact; we get:
  $\mathscr{L}[t^2] = \dfrac{2}{s}\mathscr{L}[t] = \dfrac{2}{s}\cdot
  \dfrac{1}{s^2} = \dfrac{2}{s^3}$.


- similarly $\mathscr{L}[t^3] = \dfrac{3}{s}\mathscr{L}[t^2] =
  \dfrac{3}{s} \cdot \dfrac{2}{s^3} = \dfrac{3!}{s^4}$.

- we find the general formula $\mathscr{L}[t^n] = \dfrac{n!}{s^{n+1}}$.

:::

## Computing the Laplace transform

::: incremental

- important fact: the Laplace transform is *linear*. 

- this means: for functions $f(t)$ and $g(t)$ and for constants
  $k$, we have $$\mathscr{L}[f(t) + g(t)] = \mathscr{L}[f(t)] +
  \mathscr{L}[g(t)] \quad
  \text{and} \quad
  \mathscr{L}[kf(t)] = k \mathscr{L}[f(t)].$$

- combining this with our formulas, we can compute many Laplace transforms.

- e.g.

  $$\mathscr{L}[t^3 + e^{2t} - 3\cos(5t)] = 
  \mathscr{L}[t^3]  + \mathscr{L}[e^{2t}] - 3\mathscr{L}[\cos(5t)]
  = \dfrac{3!}{s^4} + \dfrac{1}{s-2} -3\dfrac{s}{s^2 + 25}$$

:::

## (First) Differentiation Formula

::: incremental

- the reason we are interested in the Laplace transform is that it
  will permit us to solve some initial value problems.
  
- as a starting point for understanding why $\mathscr{L}$ is useful in
  this regard, we note the following important fact, which in the text
  [@gutermanNitecki, \S 5.3] is the first case of the the *First
  Differentiation Formula*:
  
  For a function $x = x(t)$, we have
  $$\mathscr{L}[Dx] = s\mathscr{L}[x] - x(0).$$

:::

-----

::: incremental

- to see why the formula $\mathscr{L}[Dx] = s\mathscr{L}[x] - x(0)$ holds, notice that

  $$\mathscr{L}[x'(t)]  = \lim_{h \to \infty} \int_0^h e^{-st} x'(t)dt \quad (\clubsuit)$$

- we may integrate by parts using $u = e^{-st}$ and $dv = x'(t)dt$. We get:

  \begin{align*}
  (\clubsuit) \quad &= \lim_{h \to \infty} \left(e^{-st} x(t) \bigg
  \vert^h_0 + s\int_0^h e^{-st} x(t)\right) \\
  &= \lim_{h \to \infty} e^{-sh}x(h) - x(0) + s\mathscr{L}[x(t)]
  \end{align*}
  
  Since $\lim_{h \to \infty} e^{-sh}x(h)  = 0$, the indicated formula holds.

:::

## Higher derivatives

::: incremental

- Next notice that 
  \begin{align*}
  \mathscr{L}[D^2x] &= \mathscr{L}[Dx'(t)] =
  s\mathscr{L}[x'(t)] - x'(0) \\
  &= s(s\mathscr{L}[x(t)] - x(0)) - x'(0) \\
  &= s^2 \mathscr{L}[x(t)] - s x(0) - x'(0)  
  \end{align*}

- More generally, we find that

  $$\mathscr{L}[D^kx] = s^k \mathscr{L}[x(t)] - s^{k-1}x(0) - s^{k-2}x'(0) - \cdots - s x^{(k-2)}(0) - x^{(k-1)}(0).$$

:::


## Example

Use the differentiation formula to find an expression for
$\mathscr{L}[x]$ where $x$ is a solution to the initial value problem
$$(D^2 + 1)x = e^{-2t}, \quad x(0) = x'(0) = 0.$$

::: incremental

- apply $\mathscr{L}$ to each side of the ODE to get
  $$\mathscr{L}[D^2x] + \mathscr{L}[x] = \mathscr{L}[e^{-2t}].$$

- now use the differentiation formula to get
  $$s^2\mathscr{L}[x] - sx(0) - x'(0) + \mathscr{L}[x] = \dfrac{1}{s+2}.$$

::: 

----

::: incremental

- substitution of $x(0) = 0$ and $x'(0)= 0$ now gives
  $$s^2\mathscr{L}[x] + \mathscr{L}[x] = \dfrac{1}{s+2}$$
  or
  $$(s^2+1)\mathscr{L}[x] = \dfrac{1}{s+2}$$

- thus
  $$\mathscr{L}[x] = \dfrac{1}{(s+2)(s^2+1)}.$$
  
- our goal is to find $x$.  A typical strategy is to use partial
  fractions to rewrite the RHS in order to recognize the terms as
  Laplace transforms. We'll describe below this process ("inverse
  Laplace transforms")

::: 


---

::: incremental

- see [@gutermanNitecki \S 5.3 page 430-431] for some useful *notes* on partial fractions

- let's carry out partial fractions on the RHS of

  $$\mathscr{L}[x] = \dfrac{1}{(s+2)(s^2+1)}.$$

- we write

  $$\dfrac{1}{(s+2)(s^2+1)} = \dfrac{A}{s+2} + \dfrac{Bs + C}{s^2 + 1}.$$
  
- and we find

  $$\dfrac{1}{(s+2)(s^2+1)} = \dfrac{A(s^2+1) + (Bs + C)(s+2)}{(s+2)(s^2 + 1)}.$$
  
  and thus
  
    $$1 = A(s^2+1) + (Bs + C)(s+2).$$

:::

----

::: incremental

- evaluate $1 = A(s^2+1) + (Bs + C)(s+2)$ at 3 different values of $s$
  to get equations for $A,B,C$.

  e.g. $s=-2$, $s=0$, $s=1$

- $s=-2$ gives: $1 = 5A$

- $s=0$ gives $1 = A + 2C$.

- $s=1$ gives $1 = 2A + 3B + 3C$.

- to solve this system of equations, perform row operations on the
  augmented matrix:

  \begin{align*}
  \left[\begin{array}{c|c}
  \begin{matrix} 5 & 0 & 0 \\
  1 & 0 & 2 \\
  2 & 3 & 3 \\
  \end{matrix} &
  \begin{matrix}1 \\ 1 \\ 1
  \end{matrix}
  \end{array}\right]
  &\sim 
  \left[\begin{array}{c|c}
  \begin{matrix} 1 & 0 & 0 \\
  2 & 3 & 3 \\  
  1 & 0 & 2 \\
  \end{matrix} &
  \begin{matrix}1/5 \\ 1 \\ 1
  \end{matrix}
  \end{array}\right]
  \sim 
  \left[\begin{array}{c|c}
  \begin{matrix} 1 & 0 & 0 \\
  0 & 3 & 3 \\  
  0 & 0 & 2 \\
  \end{matrix} &
  \begin{matrix}1/5 \\ 3/5 \\ 4/5
  \end{matrix}
  \end{array}\right]  \\ 
  &\sim 
  \left[\begin{array}{c|c}
  \begin{matrix} 1 & 0 & 0 \\
  0 & 1 & 1 \\  
  0 & 0 & 1 \\
  \end{matrix} &
  \begin{matrix}1/5 \\ 1/5 \\ 2/5
  \end{matrix}
  \end{array}\right]    
  \sim 
  \left[\begin{array}{c|c}
  \begin{matrix} 1 & 0 & 0 \\
  0 & 1 & 0 \\  
  0 & 0 & 1 \\
  \end{matrix} &
  \begin{matrix}1/5 \\ -1/5 \\ 2/5
  \end{matrix}
  \end{array}\right]      
  \end{align*}
  

:::

----

::: incremental

- thus $A= 1/5$, $B=-1/5$ and $C=2/5$.

- so we find that
  \begin{align*}
  \dfrac{1}{(s+2)(s^2+1)} &= \dfrac{A}{s+2} + \dfrac{Bs + C}{s^2 + 1}
  = \dfrac{1}{5}\left(\dfrac{1}{s+2} + \dfrac{-s + 2}{s^2 + 1}\right) \\
  &= \dfrac{1}{5}\left(\dfrac{1}{s+2} + \dfrac{-s}{s^2 + 1} 
  + \dfrac{2}{s^2 + 1}\right).
  \end{align*}

- here is now the point: we *recognize* that 
  $\dfrac{1}{s+2}$ is the Laplace transform of $e^{-2t}$
  
- that $\dfrac{s}{s^2+1}$ is the Laplace transform of $\cos(t)$.

- and that $\dfrac{1}{s^2+1}$ is the Laplace transform of $\sin(t)$.

- we conclude that

  $$x(t) = \dfrac{1}{5}\left(e^{-2t} - \cos(t) + 2\sin(t)\right)$$

:::


## The Inverse Laplace transform

::: incremental

- if $\mathscr{L}[f(t)] = F(s)$, we say that $\mathscr{L}^{-1}[F(s)] = f(t)$.

- Thus $\mathscr{L}^{-1}$ is a transformation whose *input* is
  a function of $s$, and whose *output* is a function of $t$.
  
- we've seen that $\mathscr{L}[e^{-t}] = \dfrac{1}{s+1}$. Thus,
  $\mathscr{L}^{-1}\left[\dfrac{1}{s+1}\right] = e^{-t}$.

- similarly, we've seen that $\mathscr{L}[t^4] = \dfrac{4!}{s^5} = \dfrac{24}{s^5}$.
  
- Thus (using the linearity of $\mathscr{L}$ and $\mathscr{L}^{-1}$) we find
  $$\mathscr{L}^{-1}\left[\dfrac{1}{s^5}\right] = \dfrac{t^4}{24}.$$

:::

## Basic inverse Laplace transforms


- $\mathscr{L}^{-1}\left[\dfrac{1}{s-\lambda}\right] =  e^{\lambda t}$
- $\mathscr{L}^{-1}\left[\dfrac{1}{s}\right] = 1$
- $\mathscr{L}^{-1}\left[\dfrac{1}{s^{n+1}}\right]  = \dfrac{t^n}{n!}$
- $\mathscr{L}^{-1}\left[\dfrac{1}{s^2 + \beta^2}\right] = \dfrac{1}{\beta} \sin(\beta t)$
- $\mathscr{L}^{-1}\left[\dfrac{s}{s^2 + \beta^2}\right] = \cos(\beta t)$






## Appendix

## check: $\mathscr{L}[\cos(\beta t)]$

$$\mathscr{L}[\cos(\beta t)] = \lim_{h \to \infty} \int_0^h e^{-st} \cos(\beta t) dt.$$

::: incremental


- Now integration by parts with $u = e^{-st}$ and $dv = \cos(\beta
  t)dt$ gives $$\int_0^h e^{st} \cos(\beta t) dt = \dfrac{e^{-st}
  \sin(\beta t)}{\beta}\bigg \vert^{t=h}_{t=0}
  + \dfrac{s}{\beta} \int_0^h e^{-st} \sin(\beta t)dt \quad (\diamondsuit)$$


- Integration by parts again, this time with $U = e^{-st}$ and $dV =
  \sin(\beta t)dt$ gives $$\int_0^h e^{-st} \sin(\beta t)dt =
  \dfrac{-e^{-st} \cos(\beta t)}{\beta}\bigg\vert^{t=h}_{t=0} -
  \dfrac{s}{\beta}\int_0^h e^{-st}\cos(\beta t) dt$$

- Plugging this back into $(\diamondsuit)$ we get: $$\int_0^h e^{st}
  \cos(\beta t) dt= \dfrac{e^{-st} \sin(\beta t)}{\beta}\bigg
  \vert^{t=h}_{t=0}
  + \dfrac{-se^{-st} \cos(\beta t)}{\beta^2}\bigg\vert^{t=h}_{t=0}
  - \dfrac{s^2}{\beta^2} \int_0^h e^{st} \cos(\beta t) dt$$

:::

-----

::: incremental

- We now get 

  \begin{align*} (1 + \dfrac{s^2}{\beta^2})\int_0^h e^{st} \cos(\beta
  t) dt &= \dfrac{e^{-st} \sin(\beta t)}{\beta}\bigg
  \vert^{t=h}_{t=0} + \dfrac{-se^{-st} \cos(\beta t)}{\beta^2}\bigg
  \vert^{t=h}_{t=0} \\ &=\dfrac{e^{-sh} \sin(\beta h)}{\beta} +
  \dfrac{- se^{-sh} \cos(\beta h) + s}{\beta^2} 
  \end{align*}


- Now for $s>0$, we know that $\displaystyle \lim_{h \to \infty}
  e^{-sh} = 0$ so we conclude that $$(\dfrac{\beta^2 +
  s^2}{\beta^2})\int_0^\infty e^{st} \cos(\beta t) dt =
  \dfrac{s}{\beta^2}$$

- This shows that $$\mathscr{L}[\cos(\beta t)](s) = \int_0^\infty
  e^{st} \cos(\beta t) dt = \dfrac{s}{\beta^2} \cdot
  \dfrac{\beta^2}{\beta^2 + s^2} = \dfrac{s}{\beta^2 + s^2}$$

:::

## More examples of partial fractions

::: incremental

- see [@gutermanNitecki \S 5.3 page 430-431] for some useful *notes* on partial fractions

- Let's use these ideas to compute $\mathscr{L}^{-1}\left[ \dfrac{1}{(s-1)(s^2+4)} \right]$

- Since $s^2+4$ is an *irreducible quadratic* (it has no real root),
  we use partial fractions as follows:
  
  $$\dfrac{1}{(s-1)(s^2+4)}  = \dfrac{A}{s-1} + \dfrac{Bs + C}{s^2 + 4}.$$

- so we need 
  \begin{align*}
  1 &= A(s^2 + 4) + (Bs + C)(s-1) \\ &= As^2 + 4A + Bs^2 - Bs + Cs - C \\
  &= (A+B)s^2 +(C-B)s + (4A-C)
  \end{align*}

:::

----

::: incremental

- comparing coefficients of $s^2$, $s$ and $1 =s^0$ in the equation
  $$1 = (A+B)s^2 +(C-B)s + (4A-C)$$
  we get three linear equations in $A,B,C$:
  
- $\left \{ \begin{matrix} A+B = 0 \\ C-B = 0 \\ 4A-C = 1 \end{matrix} \right.$  

- we consider the augmented matrix
  $$\left[\begin{array}{c|c}
  \begin{matrix} 1 & 1 & 0 \\ 0 & -1 & 1 \\ 4 & 0 &  -1  \end{matrix} & 
  \begin{matrix} 0 \\ 0 \\ 1 \end{matrix}
  \end{array}\right]
  \sim 
  \left[\begin{array}{c|c}
  \begin{matrix} 
  1 & 1 & 0 \\ 
  0 & 1 & -1 \\ 
  0 & -4 &  -1  \end{matrix} & 
  \begin{matrix} 0 \\ 0 \\ 1 \end{matrix}
  \end{array}\right]
  \sim 
  \left[\begin{array}{c|c}
  \begin{matrix} 
  1 & 1 & 0 \\ 
  0 & 1 & -1 \\ 
  0 & 0 &  -5  \end{matrix} & 
  \begin{matrix} 0 \\ 0 \\ 1 \end{matrix}
  \end{array}\right]  
  $$

- we now see that $C = \dfrac{-1}{5}$, $B = C = \dfrac{-1}{5}$ and $A = -B = \dfrac{1}{5}$.

:::

----

::: incremental

- recall that
  $$\dfrac{1}{(s-1)(s^2+4)}  = \dfrac{A}{s-1} + \dfrac{Bs + C}{s^2 + 4}.$$

- and that $C = \dfrac{-1}{5}$, $B = \dfrac{-1}{5}$ and $A = \dfrac{1}{5}$.

- Thus we see that 
  $$\dfrac{1}{(s-1)(s^2+4)}  = \dfrac{1/5}{s-1} + \dfrac{-s/5 + -1/5}{s^2 + 4}
  = \dfrac{1}{5} \left(\dfrac{1}{s-1} - \dfrac{1+s}{s^2 + 4} \right)$$

- finally

  \begin{align*}\mathscr{L}^{-1}\left[\dfrac{1}{(s-1)(s^2+4)}\right]
  &= \dfrac{1}{5} \left(\mathscr{L}^{-1}\left[\dfrac{1}{s-1}\right] 
  - \mathscr{L}^{-1}\left[\dfrac{s}{s^2+4} \right]
  - \mathscr{L}^{-1}\left[\dfrac{1}{s^2+4} \right] \right)\\
  &= \dfrac{1}{5}\left(e^{t}  - \cos(2t) - \dfrac{\sin(2t)}{2}\right)  
  \end{align*}

:::

## Another example

- Let's carry out partial fractions on $\dfrac{1}{(s+2)(s-1)(s+1)}$.
  We write:

  $$\dfrac{1}{(s+2)(s-1)(s+1)} = \dfrac{A}{s+2} + \dfrac{B}{s-1} + \dfrac{C}{s+1}.$$

- getting a common denominator, we find that

  \begin{align*}
  1 &= A(s-1)(s+1) + B(s+2)(s+1) + C(s+2)(s-1) \\
  &= A(s^2 -1) + B(s^2 + 3s + 2) + C(s^2 +s -2) \\
  &= (A+B+C)s^2 + (3B + C)s + (-A + 2B - 2C)
  \end{align*}

- comparing coefficients, we get three equations:

  $$\left\{ 
  \begin{matrix}
  A + B + C  &= 0 \\
  3B + C &= 0 \\
  -A + 2B - 2C &= 1
  \end{matrix}
  \right .$$
:::



---

::: incremental

- consider the augmented matrix
  $$\left[
  \begin{array}{c|c}
  \begin{matrix}
  1 & 1 & 1 \\
  0 & 3 & 1 \\
  -1 & 2 & -2 
  \end{matrix} & 
  \begin{matrix} 0 \\ 0 \\ 1
  \end{matrix}   
  \end{array}
  \right]
  \sim 
  \left[
  \begin{array}{c|c}
  \begin{matrix}
  1 & 1 & 1 \\
  0 & 3 & 1 \\
  0 & 3 & -1 
  \end{matrix} & 
  \begin{matrix} 0 \\ 0 \\ 1
  \end{matrix}   
  \end{array}
  \right]
  \sim
  \left[
  \begin{array}{c|c}
  \begin{matrix}
  1 & 1 & 1 \\
  0 & 0 & 2 \\
  0 & 3 & -1 
  \end{matrix} & 
  \begin{matrix} 0 \\ -1 \\ 1
  \end{matrix}   
  \end{array}
  \right]
    \sim
  \left[
  \begin{array}{c|c}
  \begin{matrix}
  1 & 1 & 1 \\
  0 & 3 & -1 \\
  0 & 0 & 1 \\
  \end{matrix} & 
  \begin{matrix} 0 \\ 1 \\ -1/2
  \end{matrix}   
  \end{array}
  \right] 
  \sim
  $$

  $$
  \left[
  \begin{array}{c|c}
  \begin{matrix}
  1 & 1 & 0 \\
  0 & 3 & 0 \\
  0 & 0 & 1 \\
  \end{matrix} & 
  \begin{matrix} 1/2 \\ 1/2 \\ -1/2
  \end{matrix}   
  \end{array}
  \right] 
  \sim
  \left[
  \begin{array}{c|c}
  \begin{matrix}
  1 & 1 & 0 \\
  0 & 1 & 0 \\
  0 & 0 & 1 \\
  \end{matrix} & 
  \begin{matrix} 1/2 \\ 1/6 \\ -1/2
  \end{matrix}   
  \end{array}
  \right] 
  \sim
  \left[
  \begin{array}{c|c}
  \begin{matrix}
  1 & 0 & 0 \\
  0 & 1 & 0 \\
  0 & 0 & 1 \\
  \end{matrix} & 
  \begin{matrix} 1/3\\ 1/6 \\ -1/2
  \end{matrix}   
  \end{array}
  \right]   
  $$

- thus $A=1/3$, $B = 1/6$ and $C=-1/2$.
  
- recall that
  $\dfrac{1}{(s+2)(s-1)(s+1)} = \dfrac{A}{s+2} + \dfrac{B}{s-1} + \dfrac{C}{s+1}.$

- so we conclude $\dfrac{1}{(s+2)(s-1)(s+1)} =
  \dfrac{1}{3}\cdot\dfrac{1}{s+2} + \dfrac{1}{2}\cdot\dfrac{1}{s-1} +
  \dfrac{-1}{2}\cdot\dfrac{1}{s+1}.$
  
:::



## Bibliography {.unnumbered}

::: {.refs}
:::
