---
author: Math 51 Fall 2021
title: |
  Problem Set 4 \
  Linear Independence; Constant Coefficient Linear ODES (real roots)
date: due 2022-02-14 at 11:00 PM
bibliography: 
 - /home/george/Prof-Math/assets/math-bibliography.bib
 - /home/george/Prof-Math/assets/teaching.bib 
csl: assets/chicago-author-date.csl
header-includes: |
  \usepackage[top=25mm,bottom=25mm,left=25mm,right=25mm]{geometry}
  \usepackage{palatino,mathpazo}
---

**Reminders**

- Midterm 1 is February 14 in the *open block* -- 12:00-1:20 PM.

-----

These problems cover [@gutermanNitecki, secs. 2.4, 2.5]

#. Decide whether the  indicated functions are linearly independent on the interval $(-\infty,\infty)$.
   If the functions are linearly independent, show that this is the
   case using the definition, or using the Wronskian test. To show
   that the functions $f_1(t),f_2(t),\dots,f_n(t)$ are linearly
   dependent, you need to give explicit values $c_1,c_2,\cdots,c_n$
   for which at least one $c_i$ is non-zero and such that $0 = c_1
   h_1(t) + c_2 h_2(t) + \cdots + c_n h_n(t)$ for every $t$.

   a. $h_1(t) = 1, \quad h_2(t) = t-2, \quad h_3(t) = (t-2)^2$.

   b. $h_1(t) = t^5, \quad h_2(t) = |t^5|$.

   c. $h_1(t) = \sin^2(t) + 1, \quad h_2(t) = 2\cos^2(t), \quad h_3(t) = 10$
   
   d. $h_1(t) = e^t, \quad h_2(t) = e^{t+1}, \quad h_3(t) = 1.$
   
#. Suppose that $h_1(t), h_2(t), h_3(t)$ are linearly dependent. Show that
   $h_1'(t),h_2'(t),h_3'(t)$ are linearly dependent, as well.
   
   You will need to use the *definition* of linear dependence to make
   this argument.
   
#. Find the general solution of each of the following ODEs:

   a. $(D^2-2)(D+4)^2 x = 0$

   b. $D(D^2 - 4)^2x=0$.
   
   c. $\dfrac{d^2x}{dt^2} - 2\dfrac{dx}{dt} - 4x = 0$.

#. Solve the initial value problem $$(D+2)^2 D x = 0; \quad x(0) = x'(0) =  1, \quad 
   x''(0) = 0.$$

#. Use the exponential shift formula (see the reminder below) to compute
   the function $Lf = L[f]$ in each case:

   a. $L = D^2 + D - 1, \quad f(t) = e^t\sin(t)$
   
   b. $L = (D-1)(D^2 + D + 1), \quad f(t) = te^{2t}$.
   


### Exponential shift formula {.unnumbered}

  Recall: the *exponential shift formula* shows that for a polynomial
  $P(r)$, application of the corresponding differential operator
  $P(D)$ to the product $e^{\lambda t}y$ for a function $y$ yields
	  
  $$P(D)[e^{\lambda t}y] = e^{\lambda t}P(D+\lambda)[y]$$




# Bibliography {.unnumbered}

:::{#refs}
:::
