---
author: Math 51 Fall 2021
title: |
  Problem Set 6 \
  Complex Roots and Undetermined Coefficients
date: due 2021-10-24 at 11:59 PM
bibliography: /home/george/Prof-Math/assets/math-bibliography.bib
csl: assets/chicago-author-date.csl
header-includes: |
  \usepackage[top=25mm,bottom=25mm,left=25mm,right=25mm]{geometry}
  \usepackage{palatino,mathpazo}
---

These problems concern [@gutermanNitecki § 2.6, 2.7 ].

#. Find the general solution to the ODE
   $$x^{(4)} - x^{(2)} - 6x = 0.$$
   
   **Suggestion:** You can factor $r^4 - r^2 - 6$ by setting $u=r^2$
   and first factoring $u^2 - u - 6$.

   :::{.solution}
   \color{red}
   **Solution:**

   Since $u^2 - u - 6 = (u-3)(u+2)$, we find that $$r^4 - r^2 - 6 =
   (r^2 -3)(r^2 +2) =
   (r-\sqrt{3})(r+\sqrt{3})(r-i\sqrt{2})(r+i\sqrt{2}).$$

   Thus, the general solution to the ODE is given by
   $$x(t) = c_1 e^{\sqrt{3}t} + c_2 e^{-\sqrt{3}t} + c_3 \cos(\sqrt{2}t) + c_4 \sin(\sqrt{2}t).$$

   -----
   
   \color{black}
   :::


#. Find a polynomial differential operator $A(D)$ for which
   $A(D)[y] = 0$ for the indicated functions $y = y(t)$. Choose your
   $A(D)$ to have the *smallest possible order*.

   a. $y = 3e^t - \cos(5t) + t$.

      :::{.solution}
      \color{red}
      **Solution:**
   
      $A(D) = (D-1)\cdot (D^2 + 25)\cdot D^2$.
      
      -----
      
      \color{black}
      :::
   

   b. $y = e^t\sin(2t) - 2te^t\cos(2t) + \sin(\pi t)$. 
   
      :::{.solution}
      \color{red}
      **Solution:**
   
      $A(D) = [(D - (1+2i))\cdot (D - (1-2i))]^2\cdot (D^2 + \pi^2) = (D^2 - 2D + 5)^2 \cdot (D^2 + \pi^2)$.
   
      -----
      
      \color{black}
      :::
   

#. Make a *simplified guess*  for a particular solution to the ODE
   $$(D−1)^2(D^2+1)(D+2)x=t^2e^{3t}+e^t−t\sin(t).$$

   Note: You aren't required to *solve for the coefficients*

   :::{.solution}
   \color{red}
   **Solution:**
   
   We first find an operator $A(D)$ for which $A(D)[t^2e^{3t}+e^t−t\sin(t)] = 0$.
   
   The operator with smallest order with this property is
   
   $$A(D) = (D-3)^3\cdot(D-1)\cdot (D^2 + 1)^2.$$
   
   So we can construct an *unsimplified* guess for a particular solution by looking
   at solutions to the auxiliary homogeneous ODE
   
   $$0 = A(D)(D-1)^2(D^2+1)(D+2) = (D-3)^3(D-1)^3(D^2+1)^3(D+2).$$
   
   The general solution to this auxiliary ODE is generated by
   $$e^{3t}, \quad te^{3t}, \quad t^2e^{3t}, \quad e^t, \quad te^t, \quad t^2 e^t \quad 
   \cos(t), \quad \sin(t), \quad t\cos(t), \quad t\sin(t), \quad t^2\cos(t), 
   \quad t^2\sin(t), \quad e^{-2t}$$

   We now consider the question: among these 13 functions, which are
   solutions to the homogeneous equation corresponding to the
   *original ODE*. I.e.  which ones are solutions to
   
   $$(D−1)^2(D^2+1)(D+2)x = 0.$$

   The answer is:
   
   $$e^t, \quad te^t, \quad \cos(t), \quad \sin(t), \quad e^{-2t}$$
   
   Thus our simplified guess has the form
   
   $$q(t) = k_1 e^{3t} + k_2 te^{3t} + k_3 t^2e^{3t} +  k_4 t^2e^t +  k_5 t\cos(t) + k_6 t\sin(t) 
   + k_7 t^2 \cos(t) + k_8 t^2 \sin(t).$$

   **Note:** This is **not** a *general solution* -- in order to find
   a particular solution to the given inhomogeneous ODE, one would
   need to *solve for $k_1,k_2,\cdots$*!

   -----
   
   \color{black}
   :::


#. Solve the initial value problem
   $$(D^3−2D^2+2D−4)x=0; \quad x(0) = 0,x'(0) =4,x''(0) =12.$$

   **Suggestion:** First find the general solution. To do this, notice
   that $\lambda = 2$ is a root of the polynomial $r^3 - 2r^2 +2r -
   4$. Now use *long division of polynomials*
   
   $$ r-2 \big \vert \overline{\,r^3 - 2r^2 + 2r - 4};$$

   this will permit you to write $r^3 - 2r^2 + 2r - 4 = (r-2)Q(r)$ for
   some quadratic polynomial $Q(r)$. After you factor $Q(r)$, you'll
   know all the roots to $r^3 - 2r^2 +2r - 4$.

   :::{.solution}
   \color{red}
   **Solution:**

   Using long division, you'll find that
   
   $$r^3 -2r^2 +2r -4 = (r-2)(r^2 +2) = (r-2)(r-\sqrt{2}i)(r+\sqrt{2}i).$$
   
   Thus the *general solution* to the homogeneous ODE is given by
   
   $$x(t) = c_1 e^{2t} + c_2\cos(\sqrt{2}t) + c_3 \sin(\sqrt{2}t).$$

   Let's observe that
   $$x'(t) = 2c_1 e^{2t} -c_2 \sqrt{2} \sin(\sqrt{2}t) + c_3 \sqrt{2} \cos(\sqrt{2}t).$$
   and
   $$x''(t) = 4c_1 e^{2t} - 2 c_2\cos(\sqrt{2}t) - 2 c_3 \sin(\sqrt{2}t).$$
   
   To solve the initial value problem, we need:
   $$0 = x(0) = c_1 + c_2.$$
   $$4 = x'(0) = 2c_1 + c_3 \sqrt{2}.$$
   $$12 = x''(0) = 4c_1 - 2c_2.$$ 
   
   The first equation shows that $c_2 = -c_1$.
   Replacing $c_2$ by $-c_1$ in the third equation, we need to solve the system
   $$\left \{
   \begin{matrix}
   4 & = & 2c_1 & + & c_3 \sqrt{2} \\
   12 & = & 4c_1 & + & 2c_1 \\
   \end{matrix}
   \right .$$
   
   Since the second equation shows that $12 = 6c_1$, we find $c_1 =
   2$, $c_2 = -2$ and finally that $c_3 = 0$ (using the first equation).
   
   Thus the solution to the initial value problem is
   
   $$x(t) = 2 e^{2t}  -2\cos(\sqrt{2}t).$$
   
   -----
   
   \color{black}
   :::


#. Find the *general solution* to the ODE $$(D^3 - D^2 - 2D)x = 1 + e^{2t}.$$

   :::{.solution}
   \color{red}
   **Solution:**
   
   Observe that $$(D^3 - D^2 - 2D) = D(D^2 -D -2) = D(D-2)(D+1).$$
   
   Now, a polynomial differential operator $A(D)$ for which $A(D)[1+e^{2t}]$ is
   $$A(D) = D(D-2).$$
   
   Thus, we find a guess for a particular solution $q(t)$ to
   $(\clubsuit) \quad (D^3 - D^2 -2D)x = 1 + e^{2t}$ from among the
   solutions to the auxiliary homogeneous equation $$0=A(D) \cdot
   (D^3 - D^2 - 2D)x = D(D-2)(D^3 - D^2 - 2D) = D^2 (D-2)^2 (D+1)$$
   The solution to this auxiliary homog equation is generated by $$1,
   \quad t, \quad e^{2t}, \quad te^{2t}, \quad e^{-t}.$$ Of these
   functions, $1$, $e^{2t}$ and $e^{-t}$ are already solutions to the
   homogeneous equation $(D^3 - D^2 -2D)x=0$ and hence we may and will
   discard them.
   
   Thus our *simplified guess* for the particular solution is
   
   $$q(t) = k_1 t + k_2 te^{2t}.$$
   
   We must now solve for $k_1,k_2$. For this, we must compute
   $$(D^3 - D^2 -2D)[k_1 t + k_2te^{2t}].$$
   
   We have $(D^3 - D^2 - 2D)[t] = -2$ and using the *exponential shift
   formula* we find that
   \begin{align*}
   (D^3 - D^2 - 2D)[te^{2t}] &= e^{2t} ((D+2)^3 -(D+2)^2 - 2(D+2))[t] \\
   &= e^{2t} (D^3 + 6D^2 + 12D + 8 - D^2 - 4D - 4 - 2D -4))[t] \\
   &= e^{2t} (D^3  + 5D^2 + 6D ))[t]  \\
   &= 6e^{2t}.
   \end{align*}
   
   This shows that
   
   $$(D^3 - D^2 -2D)[k_1 t + k_2te^{2t}] = -2k_1 + 6 k_2e^{2t}.$$
   
   So in order to arrange that $q(t) = k_1 t + k_2te^{2t}$ is a
   particular solution to $(\clubsuit)$, we need that $$-2k_1 +
   +6k_2e^{2t} = 1 + e^{2t}.$$
   
   Comparing coefficients, we find that
   $$-2k_1 = 1 \quad \text{and} \quad 6k_2 = 1.$$
   
   Thus $k_1 = -1/2$ and $k_2= 1/6$ so the particular solution is
   $$q(t) = \dfrac{te^{2t} - 3t}{6}.$$
   
   Now, the general solution to $(\clubsuit)$ has the form $$x(t) =
   q(t) + H(t)$$ where $H(t)$ is the general solution to the
   corresponding homogeneous equation.  Thus $$x(t) = \dfrac{te^{2t} -
   3t}{6} + c_1 + c_2 e^{2t} + c_3 e^{-t}$$ is the general solution to
   $(\clubsuit)$.
   
   -----
   
   \color{black}
   :::

#. Solve the initial value problem:
   $$(D^2 - 9)x = 9 + 12e^{-3t}; \quad x(0) = x'(0) = 0.$$

   :::{.solution}
   \color{red}
   **Solution:**

   We first note that the operator
   $$A(D) = D(D-3)$$
   satisfies
   $$A(D)[9 + 12e^{-3t}] = 0.$$
   
   Thus we may look for a *particular solution* $q(t)$ to
   $$(\diamondsuit) \quad (D^2 - 9)x = 9 + 12e^{-3t}$$ among the
   general solutions to the auxiliary homogeneous equation $$0 =
   A(D)(D^2-9)x = D \cdot (D-3)^2\cdot (D+3)x.$$
   
   The general solution to this auxiliary equation is generated by
   $$1, \quad e^{-3t}, \quad te^{-3t}, \quad e^{3t}.$$
   
   Among these solutions, $e^{3t}$ and $e^{-3t}$ are already solutions
   to the homogeneous equation $(D^2 + 9)x = 0$ corresponding to
   $(\diamondsuit)$. Thus we may and will omit them from our
   simplified guess.
   
   Our guess for $q(t)$ is now:
   
   $$q(t)  = k_1 + k_2 te^{-3t}.$$
   
   We must find $k_1,k_2$ for which $(D^2-9)[q(t)] = 9 + 12e^{-3t}$.
   
   We compute, using the *exponential shift formula* when neeeded:
   $$(D^2-9)[1] = -9$$
   
   \begin{align*}
   (D^2-9)[te^{-3t}] &= e^{-3t} ((D-3)^2 - 9)[t] \\
   &= e^{-3t} (D^2 - 6D + 9 - 9)[t] \\
   &= e^{-3t} (D^2 - 6D)[t] \\      
   &= -6e^{-3t}
   \end{align*}

   We conclude that
   $$(D^2 -9)[k_1  + k_2 te^{-3t}] = -9k_1 - 6k_2e^{-3t}$$

   Thus, in order to arrange that $q(t)$ is a particular solution to $(\diamondsuit)$,
   we need
   $$-9k_1 - 6k_2e^{-3t} = 9 + 12e^{-3t}$$
   
   Comparing coefficients, we find that $$k_1 = -1, \quad
   k_2 = -2.$$
   
   Thus
   $$q(t) = -1 - 2te^{-3t}.$$
   
   And we conclude the general solution to $(\diamondsuit)$ is given by
   
   $$x(t) = q(t) + H(t) = -1 - 2te^{-3t} + c_1e^{3t} + c_2e^{-3t}.$$
   
   Finally, we need
   $$0 = x(0) = -1 + c_1 + c_2 = -3 + c_1 + c_2$$
   and
   $$0 = x'(0)= (-2e^{-3t}(1-3t) + 3c_1e^{3t} -3c_2e^{-3t}) \bigg \vert_{t=0}
   = -2 + 3c_1 -3c_2$$
   
   So we must solve the system of equations
   $$\left\{
   \begin{matrix}
    1 & = & c_1 & + & c_2 \\
	2 & = & 3c_1 & + & -3c_2
   \end{matrix}
   \right.$$
   
   One finds that $c_1 = \dfrac{5}{6}$ and $c_2 = \dfrac{1}{6}$, so
   the solution to the initial value problem is
   
   $$x(t) = -1 - 2te^{-3t} + \dfrac{5e^{3t}}{6} + \dfrac{e^{-3t}}{6} =
   -1 + \dfrac{5e^{3t}}{6} + \dfrac{(1-12t)e^{-3t}}{6}$$

   -----
   
   \color{black}
   :::


# Bibliography {.unnumbered} 

::: {#refs} 
:::
