---
author: Math 51 Fall 2021
title: |
  Problem Set 10 - **Solutions** \
  Homogeneous systems of linear ODEs -- solutions via eigenvalues
date: due 2021-11-21 at 11:59 PM
bibliography: 
 - /home/george/Prof-Math/assets/math-bibliography.bib
 - /home/george/Prof-Math/assets/teaching.bib
csl: assets/chicago-author-date.csl
header-includes: |
  \usepackage[top=25mm,bottom=25mm,left=25mm,right=25mm]{geometry}
  \usepackage{mathtools}
---
These problems concern [@gutermanNitecki ยง3.7 & 3.8].

#. Find the general solution to the system

   $$D \begin{bmatrix} x_1 \\ x_2 \end{bmatrix}
   = \begin{bmatrix}
   0 & -1 \\
   2 & 3
   \end{bmatrix}
   \begin{bmatrix} x_1 \\ x_2 \end{bmatrix}$$

   :::{.solution}
   \color{red}  
   **Solution:**

      The characteristic polynomial of the coefficient matrix is
      $\lambda^2 - 3\lambda + 2 = (\lambda -2)(\lambda -1)$.
	  
	  A $2$-eigenvector is $\begin{bmatrix} -1 \\ 2 \end{bmatrix}$
	  and a $1$-eigenvector is $\begin{bmatrix} -1 \\ 1 \end{bmatrix}$. Since these vectors
	  are linearly independent (they are eigenvectors for distinct eigenvalues), we see that
	  the general solution to the given linear system of ODEs is given by
	  $$\mathbf{x}(t) = c_1e^{2t}\begin{bmatrix} -1 \\ 2 \end{bmatrix} +
      c_2e^t\begin{bmatrix} -1 \\ 1 \end{bmatrix}.$$

   -----
   
   \color{black}
   :::


#. Find the general solution to the system

   $$D \mathbf{x}
   = \begin{bmatrix}
   0 & 1 & 1 \\
   -2 & -2 & 1 \\
   0 & 0 & -3
   \end{bmatrix}
   \mathbf{x} $$

   :::{.solution}
   \color{red}  
   **Solution:**

   Using row-expansion on the 3rd row, we see that the characteristic
   polynomial of the coefficient matrix is $$-(\lambda + 3) \det
   \begin{bmatrix} -\lambda & 1 \\ -2 & -2-\lambda \end{bmatrix} =
   -(\lambda + 3)(\lambda^2 + 2\lambda + 2).$$ The *quadratic formula*
   shows that the roots of $\lambda^2 + 2 \lambda +2$ are $-1\pm i$,
   so the eigenvalues of the coefficient matrix are $\lambda = -3$,
   $\lambda=-1+i$, and $\lambda=-1-i$.

   To find a $-3$-eigenvector, we consider the homogeneous equation with coefficient matrix
   $$\begin{bmatrix}
   3 & 1 & 1\\
   -2 & 1 & 1 \\
   0 & 0 & 0 \\
   \end{bmatrix} \sim 
   \begin{bmatrix}
   3 & 1 & 1 \\
   -5 & 0 & 0 \\
   0 & 0 & 0
   \end{bmatrix}
   \sim 
   \begin{bmatrix}
   1 & 0 & 0 \\
   3 & 1 & 1 \\
   0 & 0 & 0
   \end{bmatrix} \sim 
   \begin{bmatrix}
   1 & 0 & 0 \\
   0 & 1 & 1 \\
   0 & 0 & 0
   \end{bmatrix}.$$
   Since the solution space is generated by $\begin{bmatrix} 0 \\ -1 \\ 1 \end{bmatrix}$,
   we find that $\mathbf{h}_1(t) = e^{-3t} \begin{bmatrix} 0 \\ -1 \\ 1 \end{bmatrix}$
   is a solution to the system of ODEs.
   
   Next we find an eigenvector for $\lambda = -1 + i$. We consider the
   homogeneous equation with coeff. matrix
   $$\begin{bmatrix}
   1-i & 1 & 1 \\
   -2 & -1 - i & 1 \\
   0 & 0 & -2 -i
   \end{bmatrix}
   \sim 
   \begin{bmatrix}
   2 & 1+i & 1+i \\
   2 & 1+i & -1 \\
   0 & 0 & 5
   \end{bmatrix}  \sim 
   \begin{bmatrix}
   2 & 1+i & 1+i \\
   0 & 0 & -2-i \\
   0 & 0 & 1
   \end{bmatrix} \sim 
   \begin{bmatrix}
   2 & 1+i & 0 \\
   0 & 0 & 1 \\
   0 & 0 & 0
   \end{bmatrix}
   $$
   We find the eigenvector $\mathbf{v} = \begin{bmatrix} -1-i \\ 2 \\ 0 \end{bmatrix}$.
   

   We next consider the complex solution
   \begin{align*}
   e^{(-1+i)t} \mathbf{v} &= e^{-t} (\cos(t) + i \sin(t))\begin{bmatrix} -1-i \\ 2 \\ 0 \end{bmatrix}
   =e^{-t}\begin{bmatrix} (\cos(t) + i\sin(t))(-1-i) \\ 2\cos(t) + 2i\sin(t) \\ 0 \end{bmatrix} \\
   &= e^{-t}\begin{bmatrix} -\cos(t) + \sin(t) - (\cos(t) +\sin(t))i \\ 2\cos(t) + 2i\sin(t) \\ 0 \end{bmatrix} \\
   &= e^{-t}\begin{bmatrix} -\cos(t) + \sin(t) \\ 2\cos(t) \\ 0 \end{bmatrix} + i e^{-t}\begin{bmatrix} -\cos(t) - \sin(t) \\ 2\sin(t) \\ 0 \end{bmatrix} 
   \end{align*}
   By taking the *real* and *imaginary* parts of this complex solution, we find two real
   solutions with linearly independent initial vectors:
   $$\mathbf{h_2}(t) = e^{-t}\begin{bmatrix} -\cos(t) + \sin(t) \\ 2\cos(t) \\ 0 \end{bmatrix}
   \quad \text{and} \quad
   \mathbf{h_3}(t) = e^{-t}\begin{bmatrix} -\cos(t) - \sin(t) \\ 2\sin(t) \\ 0 \end{bmatrix}.$$
   
   We *do not need to consider* the complex conjugate eigenvalue
   $-1-i$, since we constructed two real solutions using the
   eigenvalue $-1+i$.
   
   The general solution to the system of linear ODEs is
   $$\mathbf{x}(t) = c_1\mathbf{h}_1(t) + c_2\mathbf{h}_2(t)  + c_3\mathbf{h}_3(t)
   = c_1 e^{-3t} \begin{bmatrix} 0 \\ -1 \\ 1 \end{bmatrix}
   + c_2 e^{-t}\begin{bmatrix} -\cos(t) + \sin(t) \\ 2\cos(t) \\ 0 \end{bmatrix}
   + c_3 e^{-t}\begin{bmatrix} -\cos(t) - \sin(t) \\ 2\sin(t) \\ 0 \end{bmatrix}$$
   
   -----
   
   \color{black}
   :::


#. Find all solutions to the inhomogeneous matrix equation
   $$\begin{bmatrix}
    1 & 1 & 1 & 2 \\
	1 & 1 & 2 & 2 \\
	1 & 1 & 2 & 1
   \end{bmatrix} 
   \begin{bmatrix}
   x_1 \\ x_2 \\ x_3 \\ x_4
   \end{bmatrix}
   = 
   \begin{bmatrix}
   1 \\ 2 \\ 1
   \end{bmatrix}$$

   :::{.solution}
   \color{red}  
   **Solution:**

   Perform row operations on the *augmented matrix*:
   \begin{align*}
   \left[\begin{array}{c|c}
   \begin{matrix}
    1 & 1 & 1 & 2 \\
	1 & 1 & 2 & 2 \\
	1 & 1 & 2 & 1 
   \end{matrix} &
   \begin{matrix}
   1 \\ 2 \\ 1
   \end{matrix}
   \end{array}\right] \sim& 
   \left[\begin{array}{c|c}
   \begin{matrix}
    1 & 1 & 1 & 2 \\
	0 & 0 & 1 & 0 \\
	0 & 0 & 1 & -1 
   \end{matrix} &
   \begin{matrix}
   1 \\ 1 \\ 0
   \end{matrix}
   \end{array}\right] \sim
   \left[\begin{array}{c|c}
   \begin{matrix}
    1 & 1 & 1 & 2 \\
	0 & 0 & 1 & 0 \\
	0 & 0 & 0 & -1 
   \end{matrix} &
   \begin{matrix}
   1 \\ 1 \\ -1
   \end{matrix}
   \end{array}\right]\sim 
   \left[\begin{array}{c|c}
   \begin{matrix}
    1 & 1 & 1 & 0 \\
	0 & 0 & 1 & 0 \\
	0 & 0 & 0 & 1 
   \end{matrix} &
   \begin{matrix}
   -1 \\ 1 \\ 1
   \end{matrix}
   \end{array}\right] \\
   \sim& 
   \left[\begin{array}{c|c}
   \begin{matrix}
    1 & 1 & 0 & 0 \\
	0 & 0 & 1 & 0 \\
	0 & 0 & 0 & 1 
   \end{matrix} &
   \begin{matrix}
   -2 \\ 1 \\ 1
   \end{matrix}
   \end{array}\right]
   \end{align*}
   
   Now observe that $x_2$ is a *free variable*, that $x_4 = x_3=1$ and that
   $x_1 + x_2 = -2$.
   
   Thus $x_1 = -2 - x_2$ and we find the solutions
   $$\begin{bmatrix}
   -2  -x_2\\ x_2 \\ 1 \\ 1 \end{bmatrix}
   = \begin{bmatrix}
   -2  \\ 0 \\ 1 \\ 1 \end{bmatrix}
   + x_2 \begin{bmatrix}
   - 1 \\ 1 \\ 0 \\ 0 \end{bmatrix}$$
   
   (*Notice that the vector $\begin{bmatrix}
   - 1 \\ 1 \\ 0 \\ 0 \end{bmatrix}$
   generates the solutions to the corresponding homogeneous equation.*)
   
   -----
   
   \color{black}
   :::


#. Solve the initial value problem $D \mathbf{x} = A \mathbf{x}$ where
   $$A = \begin{bmatrix} -1 & 2 \\ -1 & 1 \end{bmatrix} \quad
   \text{and} \quad \mathbf{x}(0) = \begin{bmatrix} 1 \\ 2
   \end{bmatrix}.$$

   :::{.solution}
   \color{red}  
   **Solution:**
   
   We first find the *general solution* to $D \mathbf{x} = A \mathbf{x}$.
   The characteristic polynomial of $A$ is $(-1-\lambda)(1-\lambda) + 2 = \lambda^2 + 1$.
   Thus the eigenvalues of $A$ are $i$ and $-i$.
   
   To find an eigenvector for $\lambda = i$, we perform row operations
   on $A - i\mathbf{I_2}$:
   $$\begin{bmatrix} -1-i & 2 \\ -1 & 1 -i \end{bmatrix} \sim 
   \begin{bmatrix} 2 & (-1+i)2 \\ 1 & -1 +i \end{bmatrix}  \sim 
   \begin{bmatrix} 1 & -1 +i \\ 0 & 0 \end{bmatrix}$$
   
   We find the eigenvector $\mathbf{v} = \begin{bmatrix} 1-i \\ 1 \end{bmatrix}$.
   We consider the *complex solution*
   \begin{align*}
   e^{it} \cdot \mathbf{v} =&
   (\cos(t) + i \sin(t)) \begin{bmatrix} 1-i \\ 1 \end{bmatrix} =
   \begin{bmatrix} (\cos(t) + i \sin(t))(1-i) \\ \cos(t) + i \sin(t) \end{bmatrix}
   = \begin{bmatrix} \cos(t) + \sin(t) + i(\sin(t) - \cos(t)) \\ \cos(t) + i \sin(t) \end{bmatrix}\\
   =& \begin{bmatrix} \cos(t) + \sin(t) \\ \cos(t) \end{bmatrix}
   + i\begin{bmatrix} \sin(t) - \cos(t) \\ \sin(t) \end{bmatrix}
   \end{align*}
   Taking the *real* and *imaginary* parts, we find the solutions
   $$\mathbf{h}_1(t) = \begin{bmatrix} \cos(t) + \sin(t) \\ \cos(t) \end{bmatrix} \quad
   \text{and}
   \quad
   \mathbf{h}_2(t) = \begin{bmatrix} \sin(t) - \cos(t) \\ \sin(t) \end{bmatrix}.$$

   The general solution has the form
   $$\mathbf{x}(t) =  c_1\mathbf{h}_1(t) + c_2\mathbf{h}_2(t).$$
   Evaluating at $t=0$, we see that we must solve the equation
   $$\begin{bmatrix} 1 \\ 2
   \end{bmatrix}  =c_1\mathbf{h}_1(0) + c_2\mathbf{h}_2(0)
   = c_1\begin{bmatrix} \cos(t) + \sin(t) \\ \cos(t) \end{bmatrix}\bigg\vert_{t=0} +
   c_2\begin{bmatrix} \sin(t) - \cos(t) \\ \sin(t) \end{bmatrix} \bigg\vert_{t=0}
   = c_1 \begin{bmatrix} 1 \\ 1 \end{bmatrix} +
   c_2 \begin{bmatrix} -1 \\ 0 \end{bmatrix}$$

   Thus we consider the matrix equation
   $$\begin{bmatrix} 1 & -1 \\ 1 & 0 \end{bmatrix}
   \begin{bmatrix} c_1 \\ c_2 \end{bmatrix} =
   \begin{bmatrix} 1 \\ 2
   \end{bmatrix}.$$
   
   We solve this by performing row operations on the augmented
   matrix. (*We could use Cramer's Rule instead.*)
   
   $$\left[ \begin{array}{c|c}
   \begin{matrix} 1 & -1 \\ 1 & 0 \end{matrix} &
   \begin{matrix} 1\\ 2
   \end{matrix}
   \end{array}\right] \sim 
   \left[ \begin{array}{c|c}
   \begin{matrix} 1 & -1 \\ 0 & 1 \end{matrix} &
   \begin{matrix} 1 \\ 1
   \end{matrix}
   \end{array}\right] \sim
   \left[ \begin{array}{c|c}
   \begin{matrix} 1 & 0 \\ 0 & 1 \end{matrix} &
   \begin{matrix} 2 \\ 1
   \end{matrix}
   \end{array}\right]$$

   We now find that $c_1=2$ and $c_2=1$ so that the solution to the initial value
   problem is 
   $$\mathbf{x}_0(t) =  2\mathbf{h}_1(t) + 1\mathbf{h}_2(t) 
   = 2\begin{bmatrix} \cos(t) + \sin(t) \\ \cos(t) \end{bmatrix} +
   \begin{bmatrix} \sin(t) - \cos(t) \\ \sin(t) \end{bmatrix}
   = \begin{bmatrix} \cos(t) + 3\sin(t) \\ 2\cos(t) + \sin(t)
   \end{bmatrix}$$
   
   -----
   
   \color{black}
   :::


#. The eigenvalues of the matrix
   $A = \begin{bmatrix} 1 & 1 & 1 \\
   0 & 2 & 0 \\
   0 & 0 & 1 \end{bmatrix}$
   are $1$ and $2$. The $1$-eigenspace is generated by the vector
   $\mathbf{v} = \begin{bmatrix} 1 \\ 0 \\ 0 \end{bmatrix}$,
   and the $2$-eigenspace is generated by the vector
   $\mathbf{w} = \begin{bmatrix} 1 \\ 1 \\ 0 \end{bmatrix}$.
   
   a. Let $\mathbf{h_1}(t) = e^t \mathbf{v}$ and $\mathbf{h_2}(t) = e^{2t}
      \mathbf{w}$. Explain why $c_1 \mathbf{h_1}(t) + c_2 \mathbf{h_2}(t)$
      is a solution to $D\mathbf{x} = A\mathbf{x}$ for all $c_1,c_2$,
      but also explain why this expression is not the *general
      solution*.

      :::{.solution}
      \color{red}  
      **Solution:**
   
      Since $\mathbf{v}$ is a $1$-eigenvector and since $\mathbf{w}$
	  is a $2$-eigenvector, we may conclude that $\mathbf{h}_1(t)$ and
	  $\mathbf{h}_2(t)$ are *solutions* to the system of ODEs.
	  
	  However, since $A$ is a $3\times 3$ matrix, the general solution
	  to $D\mathbf{x} = A \mathbf{x}$ is generated by $3$ solutions
	  with linearly independent initial vector, so the two solutions
	  $\mathbf{h}_1(t)$ and $\mathbf{h}_2(t)$ can't generate the
	  general solution.
   
      -----
      
      \color{black}
      :::


   b. If $\mathbf{x}(t)$ is a solution to $D\mathbf{x} = A\mathbf{x}$
      for which $\mathbf{x}(0) = \begin{bmatrix} 1 \\ -1 \\ 0\end{bmatrix}$,
	  find scalars $c_1,c_2$ for which 
	  $$\mathbf{x}(t) = c_1 \mathbf{h_1(t)} + c_2 \mathbf{h_2}(t).$$

      :::{.solution}
      \color{red}  
      **Solution:**
   
      Evaluating at $t=0$, we must find $c_1,c_2$ for which
	  $$\begin{bmatrix} 1 \\ -1 \\ 0\end{bmatrix}
	  = \left(c_1 e^t \mathbf{v}+ c_2 e^{2t} \mathbf{w}\right)\bigg \vert_{t=0}
	  = c_1 \mathbf{v} + c_2 \mathbf{w}
	  = \begin{bmatrix} 1 & 1 \\
	  0 & 1 \\
	  0 & 0 \end{bmatrix}
	  \begin{bmatrix} c_1 \\ c_2 \end{bmatrix}.$$
   
      Examining the augmented matrix
	  $$\left[
	  \begin{array}{c|c}
	  \begin{matrix} 1 & 1 \\
	  0 & 1 \\
	  0 & 0 \end{matrix}
	  &
	  \begin{matrix} 1 \\ -1 \\ 0\end{matrix}
	  \end{array}
	  \right] \sim 
	  \left[
	  \begin{array}{c|c}
	  \begin{matrix} 1 & 0 \\
	  0 & 1 \\
	  0 & 0 \end{matrix}
	  &
	  \begin{matrix} 2 \\ -1 \\ 0\end{matrix}
	  \end{array}
	  \right]$$
	  we see that $c_1 =2$ and $c_2= -1$.
	  
      -----
      
      \color{black}
      :::


   c. If $\mathbf{x}(t)$ is a solution to $D\mathbf{x} = A\mathbf{x}$
      for which $\mathbf{x}(0)=\begin{bmatrix} 0 \\ 2 \\ 1 \end{bmatrix}$,
	  explain why there are no scalars $c_1,c_2$ for which
	  $$\mathbf{x}(t) = c_1 \mathbf{h_1}(t) + c_2 \mathbf{h_2}(t).$$

      :::{.solution}
      \color{red}  
      **Solution:**

      Evaluating at $t=0$, we must seek $c_1,c_2$ for which
	  $$\begin{bmatrix} 0 \\ 2 \\ 1\end{bmatrix}
	  = \left(c_1 e^t \mathbf{v}+ c_2 e^{2t} \mathbf{w}\right)\bigg \vert_{t=0}
	  = c_1 \mathbf{v} + c_2 \mathbf{w}
	  = \begin{bmatrix} 1 & 1 \\
	  0 & 1 \\
	  0 & 0 \end{bmatrix}
	  \begin{bmatrix} c_1 \\ c_2 \end{bmatrix}.$$
   
      Examining the augmented matrix
	  $$\left[
	  \begin{array}{c|c}
	  \begin{matrix} 1 & 1 \\
	  0 & 1 \\
	  0 & 0 \end{matrix}
	  &
	  \begin{matrix} 0 \\ 2 \\ 1\end{matrix}
	  \end{array}
	  \right]$$
	  the third row shows that this equation is *inconsistent*.
	  Indeed, this row requires that $0c_1 + 0c_2 = 1$, which is impossible.
	  
	  Thus, there are no scalars $c_1,c_2$ with the indicated property.
	  
	  *(Parenthetically, notice that in order to find a solution $\mathbf{x}(t)$ with
	  $\mathbf{x}(0) = \begin{bmatrix} 0 \\ 2 \\ 1\end{bmatrix}$ we
	  would need to first find a third solution $\mathbf{h}_3(t)$ for which
	  the initial vectors
	  $\mathbf{h_1}(0),\mathbf{h_2}(0),\mathbf{h_3}(0)$ are linearly
	  independent.)*

      -----
      
      \color{black}
      :::


## Bibliography {.unnumbered} 

::: {#refs} 
:::
