---
author: Math 51 Fall 2021
title: |
  Problem Set 7 \
  Variation of parameters & Linear systems of ODEs
date: due 2021-10-31 at 11:59 PM
bibliography: /home/george/Prof-Math/assets/teaching.bib
csl: assets/chicago-author-date.csl
header-includes: |
  \usepackage[top=25mm,bottom=25mm,left=25mm,right=25mm]{geometry}
  \usepackage{mathtools}
---

These problems concern [@gutermanNitecki §2.8 & §3.2 ].

#. Find the general solution to 

   $$x'' - 2x' + x = e^t \ln(t), \quad t>0.$$

   :::{.solution}
   \color{red}
   **Solution:**

   Since the characteristic polyomial is $r^2 - 2r + 1=(r-1)^2$, the general
   solution to the corresponding homogeneous equation is generated by
   $$h_1(t) = e^t, \quad h_2(t) = te^t.$$
   
   To solve the inhomogeneous equation, it isn't clear how to use the
   method of *undetermined coefficients* (what should $A(D)$ be?!?) So
   we use *variation of parameters*.
   
   The Wronskian matrix is given by
   $$W = W(h_1,h_2)(t) = \det \begin{bmatrix} e^t & te^t \\
   e^t & (t+1)e^t 
   \end{bmatrix}.$$

   And following the method, we need to solve the matrix equation
   
   $$W \begin{bmatrix} c_1' \\ c_2' \end{bmatrix} =
   \begin{bmatrix}
   e^t & te^t \\
   e^t & (t+1)e^t 
   \end{bmatrix} \cdot \begin{bmatrix} c_1' \\ c_2' \end{bmatrix}
   = \begin{bmatrix} 0
   \\ e^t \ln(t) \end{bmatrix}.$$
   
   We now use *Cramer's Rule* to find $c_i'$. First note that
   $\det W = (t+1)e^{2t} - te^{2t} = e^{2t}.$
   
   We now have
   $$c_1' = \dfrac{\det \begin{bmatrix}
   0 & te^t \\
   e^t\ln(t) & (t+1)e^t 
   \end{bmatrix}}{\det W} = \dfrac{-e^{2t} \ln(t) t}{e^{2t}} = -t \ln(t)$$
   
   and
   
   $$c_2' = \dfrac{\det \begin{bmatrix}
   e^t & 0 \\
   e^t & e^t\ln(t) 
   \end{bmatrix}}{\det W} - \dfrac{\ln(t)e^{2t}}{e^{2t}} = \ln(t).$$
   
   We now find the functions $c_1,c_2$ by anti-differentiation:
   $$c_1(t) = \int c_1' dt = -\int t\ln(t) dt = \dfrac{-t^2\ln(t)}{2} + \dfrac{t^2}{4} + C = 
   \dfrac{t^2(1-2\ln(t))}{4} + C$$
   (*integrate by parts* with $u = \ln(t)$ and $dv  = t$).
   
   and 
   $$c_2(t) = \int c_2' dt = \int \ln(t) dt = t\ln(t) -t + D$$
   
   Now, we only need a particular solution to the ODE, se we take
   $C = D = 0$, and we find the particular solution
   \begin{align*}
   p(t) &= c_1(t) h_1(t) + c_2(t) h_2(t)  \\
   &= \left(\dfrac{t^2(1-2\ln(t))}{4}\right)\cdot e^t + (t\ln(t) -t) \cdot te^t \\
   &= \left(\dfrac{-2\ln(t) + 1}{4}\right)\cdot t^2e^t + \dfrac{4\ln(t) -4}{4} \cdot t^2e^t \\
   &= \dfrac{2\ln(t) -3}{4}t^2e^t
   \end{align*}
   
   Now the general solution is
   $$x(t) = p(t) + k_1 e^t + k_2 te^t = \dfrac{2\ln(t) -3}{4}t^2e^t + k_1 e^t + k_2 te^t$$
   for constants $k_1,k_2$.
   
   -----
   
   \color{black}
   :::


#. Verify that $t$ and $e^t$ are solutions of the homogeneous equation corresponding to
   $$(N) \quad [(t −1)D^2 −tD + 1]x = (t −1)^2e^t, \quad t >1,$$ and find the
   general solution of the nonhomogeneous equation $(N)$.

   (Remember to put the ODE in *standard form* when using *variation of parameters*!)

   :::{.solution}
   \color{red}
   **Solution:**

   To verify that $t$ is a homogeneous solution, we compute
   $$((t-1)D^2 -tD + 1)[t] = (t-1)D^2[t] -tD[t] + t = 0 -t + t = 0$$
   and to verify that $e^t$ is a homog. solution, we compute
   $$((t-1)D^2 -tD + 1)[e^t] = (t-1)D^2[e^t] -tD[e^t] + e^t = (t-1)e^t
   -te^t + e^t =0.$$

   We are going to describe a particular solution in the form $p(t) =
   c_1(t) t + c_2(t) e^t$; we'll find the functions $c_1$ and $c_2$
   using our *Wronskian method*. In order to use this method, we need
   to first put the ODE in *standard form*. i.e.

   $$[D^2 −\dfrac{t}{t-1}D + \dfrac{1}{t-1}]x = (t −1)e^t, \quad t >1,$$

   Now let $W$ denote the Wronskian matrix
   $W = \begin{bmatrix}
   t & e^t \\
   1 & e^t
   \end{bmatrix}.$ We must solve the matrix equation
   $$W \begin{bmatrix} c_1' \\ c_2' \end{bmatrix} 
   = \begin{bmatrix} 0 \\ (t-1)e^t \end{bmatrix}$$
   (*it was this step that requires standard form!!*)
   
   Notice that $\det W = (t-1)e^t$. Now use Cramer's Rule to find
   $$c_1' = \dfrac{\det \begin{bmatrix}
   0 & e^t \\
   (t-1)e^t & e^t
   \end{bmatrix}}{(t-1)e^t} = \dfrac{-(t-1)e^{2t}}{(t-1)e^t} = -e^t$$
   and
   $$c_2' = \dfrac{\det \begin{bmatrix}
   t & 0  \\
   1 & (t-1)e^t 
   \end{bmatrix}}{(t-1)e^t} = \dfrac{t(t-1)e^{t}}{(t-1)e^t} = t.$$
   
   We find now that
   $$c_1 = \int c_1' dt = -\int e^t dt = - e^t + C$$
   and
   $$c_2 = \int c_2' dt = \int t dt = \dfrac{t^2}{2} + D$$
   Since we only need one particular solution, we may and will take $C=D=0$.
   Now our particular solution is
   
   $$p(t) = c_1 t + c_2 e^t = -te^t + \dfrac{t^2e^t}{2} = \dfrac{(t^2 - 2t)e^t}{2}$$
   and the general solution to the inhomog. ODE is
   
   $$x(t) = p(t) + k_1 t + k_2 e^t = \dfrac{(t^2 - 2t)e^t}{2} + k_1 t + k_2 e^t.$$
   
   -----
   
   \color{black}
   :::


#. For each of the following systems of ODEs, decide whether it is linear.
   For each linear systems, do also the following:
   - indicate whether it is homogeneous
   - find a matrix $A$ and a vector $\mathbf{E}$ such that the system can
     be rewritten in the form $$D \mathbf{x} = A \mathbf{x} + \mathbf{E}$$ where
     $\mathbf{x} = \begin{bmatrix} x \\ y \\ z \end{bmatrix}$ (or
     $\mathbf{x} = \begin{bmatrix} x \\ y \end{bmatrix}$).
   
   a. $\quad \left \{ \begin{matrix*}[l]
	   x' =& ty - z \\
	   y' =&  -\dfrac{x}{t} - z + 1 \\
	   z' =&  -x -t^2y + z + 2t
	  \end{matrix*} \right .$

      :::{.solution}
      \color{red}
      **Solution:**

      The system is linear, but is not homogeneous. It can be written
	  
	  $$D \begin{bmatrix} x \\ y \\ z \end{bmatrix} =
	  \begin{bmatrix} 0 & t & -1 \\
	  \dfrac{-1}{t} & 0 & -1 \\
	  -1 & -t^2 & 1
	  \end{bmatrix}
	  \begin{bmatrix} x \\ y \\ z \end{bmatrix}
	  +
	  \begin{bmatrix} 0 \\ 1 \\ 2t \end{bmatrix}$$
	  
      -----
   
      \color{black}
      :::


   b. $\quad \left \{\begin{matrix*}[l]
      x' =& 2x - 3y \\
	  y' =& 3x^2y + y + 1
      \end{matrix*} \right .$

      :::{.solution}
      \color{red}
      **Solution:**

      The system is not linear, because the dependence $y' = 3x^2y + y + 1$
	   is not linear (it involves the non-linear term $x^2 y$).

      -----
   
      \color{black}
      :::


   c. $\quad \left \{
      \begin{matrix*}[l]
	  x' =& 7x + 11y \\
	  y' =& -2x + y
	  \end{matrix*}
	  \right .$

      :::{.solution}
      \color{red}
      **Solution:**

      The system is linear and homogeneous. It can be written
	  
	  $$D \begin{bmatrix} x \\ y  \end{bmatrix} =
	  \begin{bmatrix} 7 & 11 \\
	  -2 &  1 
	  \end{bmatrix}
	  \begin{bmatrix} x \\ y  \end{bmatrix}$$


      -----
   
      \color{black}
      :::


#. Let $A = \begin{bmatrix}
    0 & 1 \\
	-1 & 0 
   \end{bmatrix}$.
   
   a. Show that $\mathbf{h_1}(t) = \begin{bmatrix} \sin(t) \\ \cos(t)
      \end{bmatrix}, \quad \mathbf{h_2}(t) = \begin{bmatrix} \cos(t)
      \\ -\sin(t) \end{bmatrix}$ are solutions to the homogeneous
      system $$D \begin{bmatrix} x\\ y \end{bmatrix} = A
      \begin{bmatrix} x\\ y \end{bmatrix}.$$
   
      :::{.solution}
      \color{red}
      **Solution:**

      To check that $\mathbf{h_1}$ is a solution, we compute
	  $$D\mathbf{h_1} = \begin{bmatrix}
	  \dfrac{d}{dt} \sin(t) \\ \dfrac{d}{dt} \cos(t)
	  \end{bmatrix}=
	  \begin{bmatrix}
	  \cos(t) \\ -\sin(t)
	  \end{bmatrix}$$
	  and
	  $$A\mathbf{h_1} = \begin{bmatrix}
      0 & 1 \\
	  -1 & 0 
	  \end{bmatrix}\begin{bmatrix} \sin(t) \\ \cos(t)
      \end{bmatrix} = 
	  \begin{bmatrix} 0 \sin(t) + 1\cos(t) \\
	  -1 \sin(t) + 0\cos(t)
      \end{bmatrix}
	  = 
	  \begin{bmatrix}
	  \cos(t) \\ -\sin(t)
	  \end{bmatrix}.$$
	  Since these expressions agree, $\mathbf{h_1}$ is a solution.


      To check that $\mathbf{h_2}$ is a solution, we compute
	  $$D\mathbf{h_2} = \begin{bmatrix}
	  \dfrac{d}{dt} \cos(t) \\ \dfrac{d}{dt}[ -\sin(t)]
	  \end{bmatrix}=
	  \begin{bmatrix}
	  -\sin(t) \\ -\cos(t)
	  \end{bmatrix}$$
	  and
	  $$A\mathbf{h_1} = \begin{bmatrix}
      0 & 1 \\
	  -1 & 0 
	  \end{bmatrix}\begin{bmatrix} \cos(t) \\ -\sin(t)
      \end{bmatrix} = 
	  \begin{bmatrix} 0 \cos(t) + 1(-\sin(t)) \\
	  -1 \cos(t) + 0(-\sin(t))
      \end{bmatrix}
	  = 
	  \begin{bmatrix}
	  -\sin(t) \\ -\cos(t)
	  \end{bmatrix}.$$
	  Since these expressions agree, $\mathbf{h_2}$ is a solution.

      -----
   
      \color{black}
      ::: 
  

   b. Show that $\mathbf{p}(t) = \begin{bmatrix} 0 \\ -t \end{bmatrix}$ is a
      *particular solution* to the inhomogeneous equation 
	  $$(\clubsuit) \quad D \begin{bmatrix} x\\ y \end{bmatrix} = A \begin{bmatrix} x\\
      y \end{bmatrix} + \begin{bmatrix} t \\ -1 \end{bmatrix}.$$

      :::{.solution}
      \color{red}
      **Solution:**

      Compute
	  $$D \mathbf{p} = \begin{bmatrix} 0 \\ -1 \end{bmatrix}$$
	  and
	  $$A \mathbf{p} + \begin{bmatrix} t \\ -1
      \end{bmatrix} = \begin{bmatrix}
      0 & 1 \\
	  -1 & 0 
	  \end{bmatrix}\begin{bmatrix} 0 \\ -t
      \end{bmatrix} + \begin{bmatrix} t \\ -1
      \end{bmatrix}=\
	  \begin{bmatrix} -t \\ 0
      \end{bmatrix} + \begin{bmatrix} t \\ -1
      \end{bmatrix} = 
	  \begin{bmatrix} 0 \\ -1
      \end{bmatrix}
	  $$

      Since these expressions are equation,  $\mathbf{p}$ is a solution to
	  $(\clubsuit)$.

      -----
   
      \color{black}
      :::


   c. Let $\mathbf{x} = \mathbf{p}(t) + c \cdot \mathbf{h_1}(t)$ for a
      constant $c$. By computing $D[\mathbf x]$ and $A \mathbf{x} +
      \begin{bmatrix} t \\ -1 \end{bmatrix}$ and comparing the
      results, confirm that $\mathbf{x}$ is a solution to
      $(\clubsuit)$ for all $c$.
   
      (**Note:** In fact, $\mathbf{x} = \mathbf{p}(t) + c_1 \mathbf{h_1}(t) + c_2
	  \mathbf{h_2}(t)$ is the *general solution* to $(\clubsuit)$; we'll
	  see how to confirm this later in class).

      :::{.solution}
      \color{red}
      **Solution:**
 
      Using **a.** and **b.** we find for any $c$ that
	  $$D[ \mathbf{p} + c\mathbf{h_1}] = D[\mathbf{p}] + cD[\mathbf{h_1}] = 
	  \left(A \mathbf{p} + \begin{bmatrix} t \\ -1 \end{bmatrix} \right) + c A \mathbf{h_1} = 
	  A [ \mathbf{p} + c\mathbf{h_1}] + \begin{bmatrix} t \\ -1 \end{bmatrix}$$
	  which confirms that $\mathbf{x} = \mathbf{p} + c\mathbf{h_1}$ is indeed a solution to
	  $(\clubsuit)$.

      (*as an aside, we know that $\mathbf{p}(t) + c_1
	  \mathbf{h_1}(t) + c_2 \mathbf{h_2}(t)$ is the general solution
	  to $(\clubsuit)$ provided that $c_1 \mathbf{h_1}(t) + c_2
	  \mathbf{h_2}(t)$ is the general solution to the homogeneous
	  equation $D \mathbf{x} = A\mathbf{x}$. For this, we need to
	  check the linear independence of the vectors $\mathbf{h_1}(0)$
	  and $\mathbf{h_2}(0)$.*)

      -----
   
      \color{black}
      :::


5. Consider the linear ODE
   $$\mathbf{(N)} \quad (D - 3)^2x = e^{3t} \quad \text{i.e.} \quad (D^2 - 6D + 9)x = e^{3t}.$$
   
   a. Find the equivalent linear system $\mathbf{(S_N)}$ of
      ODEs. Write this system in *matrix form*.

      :::{.solution}
      \color{red}
      **Solution:**

      We set $\mathbf{x} = \begin{bmatrix} x_1 \\ x_2 \end{bmatrix}$.
	  For a solution $x$ of $(\mathbf{N})$ we set $x_1 = x$ and $x_2 = x'$.

      We have that $x_1' = x_2$ and
	  $$x_2' = x'' = -9x + 6x'  + e^{3t}= -9 x_1 + 6x_2 + e^{3t}.$$
	  
	  Thus we the system in matrix form
	  $$D \begin{bmatrix} x_1 \\ x_2 \end{bmatrix} =
	  \begin{bmatrix} 0 & 1 \\ -9 & 6 \end{bmatrix}
	  \begin{bmatrix} x_1 \\ x_2 \end{bmatrix} +
	  \begin{bmatrix} 0 \\ e^{3t} \end{bmatrix}$$
	  is equivalent to $(\mathbf{N})$.
	  
      -----
   
      \color{black}
      :::


   b. Note that the general solution to the homogeneous equation
      $\mathbf{(H)} \quad (D-2)^2x =0$ is generated by $h_1(t) =
      e^{3t}$ and $h_2(t) = te^{3t}$.  Find the corresponding vector
      solutions $\mathbf{h}_1$ and $\mathbf{h}_2$ to the homogeneous
      system $\mathbf{(S_H)}$.

      :::{.solution}
      \color{red}
      **Solution:**
	  
	  $$\mathbf{h_1} =\begin{bmatrix}
	  h_1(t) \\ h_1'(t)
	  \end{bmatrix} = 
	  \begin{bmatrix}
	  e^{3t} \\
	  3e^{3t}
	  \end{bmatrix} \quad \text{and} \quad
	  \mathbf{h_2} =\begin{bmatrix}
	  h_2(t) \\ h_2'(t)
	  \end{bmatrix} = 
	  \begin{bmatrix}
	  te^{3t} \\
	  (1+3t)e^{3t}
	  \end{bmatrix}
	  $$


      -----
   
      \color{black}
      :::


   c. Find a particular solution $p(t)$ to the equation $(D-3)^2 x =
      e^{3t}$, and find the corresponding vector solution
	  $\mathbf{p}(t)$ to the system $\mathbf{(S_N)}$.

      :::{.solution}
      \color{red}
      **Solution:**

      We can use the method of *undetermined coefficients*. We take
	  $A(D) = D-3$.  The general solution to $A(D)(D-3)^2 = (D-3)^3$
	  is generated by $e^{3t}, te^{3t}, t^2e^{3t}$ but the first two
	  functions are already solutions to the homogeneous equation
	  $(\mathbf{H})$ and may be eliminated.
	  
	  Thus our simplified guess for a particular solution is $k t^2 e^{3t}$
	  and we must find the constant $k$.
	  
	  For this, we apply the operator $(D-3)^2$ and use the
	  exponential shift formula:
	  $$(D-3)^2[kt^2 e^{3t}] = ke^{3t} (D+3-3)^2[t^2] = ke^{3t} D^2 [t^2] = 2ke^{3t}.$$
	  
	  We need $2ke^{3t} = e^{3t}$ so $k = 1/2$ and our particular solution is 
	  $p(t) = \dfrac{1}{2} t^2 e^{3t}$.

      In vector form we have
	  $$\mathbf{p} = \begin{bmatrix} p(t) \\ p'(t) \end{bmatrix} =
	  \begin{bmatrix} 
	  \dfrac{1}{2} t^2 e^{3t} \\
	  e^{3t} (t + \dfrac{3}{2}t^2)
	  \end{bmatrix}
	  = e^{3t}\begin{bmatrix}
	  t^2/2 \\
	  (3t^2 + 2t)/2
	  \end{bmatrix}.$$

      -----
   
      \color{black}
      :::


   d. The general solution to $\mathbf{(N)}$ is given by $x(t) =
      p(t) + c_1 h_1(t) + c_2 h_2(t)$. Indicate the the corresponding
      solutions $\mathbf{x}$ to the system $\mathbf{(S_N)}$.

      :::{.solution}
      \color{red}
      **Solution:**

      $$\mathbf{x}  = \mathbf{p} + c_1 \mathbf{h_1} + c_2 \mathbf{h_2} 
	  = e^{3t}\begin{bmatrix}
	  t^2/2 \\
	  (3t^2 + 2t)/2
	  \end{bmatrix} +
      c_1 
	  \begin{bmatrix}
	  e^{3t} \\
	  3e^{3t}
	  \end{bmatrix}  + c_2
	  \begin{bmatrix}
	  te^{3t} \\
	  (1+3t)e^{3t}
	  \end{bmatrix}$$

      -----
   
      \color{black}
      :::


# Bibliography {.unnumbered} 

::: {#refs} 
:::
